src/codec.v
@@ -1,14 +1,24 @@
 Require Import ast_instructions.
 Require Import association_list.
 Require Import binary.
+  
+  
+(* Simple encoder for unit *)
+Definition unitEncode (l: list bool) : (unit*list bool) :=
+  (tt, l).
 
-(* Product decoding function in order to get 2 types. eg: (Opcode * arguments) *)
+(* Product decoding function in order to decode 2 kinds of data. eg: (Opcode * arguments) *)
 Fixpoint crossDecode (A B: Type) (l: list bool) (dA: list bool -> (A*list bool)) (dB: list bool -> (B*list bool)) : (A*B*list bool) :=
   match dA l with
   | (a, l') => match dB l' with
                | (b, l'') => (a,b,l'')
                end
   end.
+
+(* Decoding function using 2 given codecs *)
+Fixpoint sumDecode (A B: Type) (l: list bool) (dA: list bool -> (A*list bool)) (dB: list bool -> (B*list bool)) : (A*B*list bool) :=
+  match dA l with
+
 
 (* Returns the decoded result from a decoding function *)
 Fixpoint getResultDecode (A: Type) (l: list bool) (decode: list bool -> (A*list bool)) : A :=
@@ -25,3 +35,4 @@ Fixpoint getRemListDecode (A: Type) (l: list bool) (decode: list bool -> (A*list
 (* We want to prove the correctness of the decoding function *) 
 (* Lemma decode_composition : forall (A B: Type) (l: list bool) (dA: list bool -> (A*list bool)) (dB: list bool -> (B*list bool)),
     . *)
+    
